<?xml version="1.0" encoding="UTF-8"?>

<section xml:id="sec-week-1" xmlns:xi="http://www.w3.org/2001/XInclude">
  <title>Week 1</title>

  <p> Problems For week 1, due <alert>4pm Wednesday 9th October</alert>. </p>
  <problem>
    <title>Arc Lengths</title>    
    <p>
      Find the arc length of <m>f(x)</m>  along <m>[a,b]</m>.
      <ol marker="(a)">
        <li>
          <p>
            cosh<m>(x)</m>  along <m>[0,2]</m> 
          </p>
        </li>
        <li>
          <p>
            <m>\frac{x^4}{8} + \frac{1}{4x^2}</m>  along <m>[1,3]</m>
          </p>
        </li>
        <li>
          <p>
            <m>x^2+3x+2</m>  along <m>[0,1]</m>
          </p>
        </li>
        <li>
          <p>
            <alert>(H)</alert> <m>\frac{1}{2}</m>ln<m>(x) - \frac{1}{4}x^2</m>  along <m>[1,e]</m>
          </p>
        </li>
      </ol>
    </p>
    <hint>
      <p>
        The arc length formula is given by
        <md>
          <mrow> S = \int_a^b\sqrt{1+\bigg(\frac{dy}{dx}\bigg)^2}dx \amp </mrow>
        </md>
        The following identities are also useful
        
        <md>
          <mrow> \text{cosh}^2(x) - \text{sinh}^2(x) =\amp 1 </mrow>
          <mrow>\text{cosh}^2(x) + \text{sinh}^2(x) =\amp\text{cosh}(2x). </mrow>
        </md>
        These combine to give
        <md>
          <mrow>\text{cosh}^2(x) =\amp\frac{1}{2}(\text{cosh}(2x)+1) </mrow>
          <mrow>\text{sinh}^2(x) =\amp\frac{1}{2}(\text{cosh}(2x)-1). </mrow>
        </md>
        We also have
        <md>
          <mrow>\text{cosh}(\text{arsinh}(x)) =\amp\sqrt{x^2+1} </mrow>
          <mrow>\text{sinh}(\text{arcosh}(x)) =\amp\sqrt{x^2-1} </mrow>
        </md>
        and even
        <md>
          <mrow>\text{sin}(x) =\amp \text{sinh}(ix) </mrow>
          <mrow>\text{sinh}(x) =\amp \text{sin}(-ix) </mrow>
          <mrow>\text{cos}(x) =\amp \text{cosh}(ix) </mrow>
          <mrow>\text{cosh}(x) =\amp \text{cos}(-ix). </mrow>
        </md>
      </p>
    </hint>
    <hint>
      <title>Part (c).</title>
      <p>
        Use the substitution <m>2x + 3 = \sinh(\theta)</m>
      </p>
    </hint>
    <answer>
      <title>Part (d).</title>
      <p>
        Nobody knows.
        <!--<m>\frac{1+e^2}{4}</m>
      -->
      </p>
    </answer>
  </problem>
  <problem>
    <title>Question 3</title>
    <p>
      <alert>(H)</alert> Suppose a chain of length <m>L</m> is suspended between two points <m>x=-H</m> and <m>x=H</m>,
       both of which are at height <m>y = 1</m>.
      The shape of the chain is then given by <m>y(x)</m> with <m>y(-H) = y(H) = 1</m>.
      Assume the lowest part of the hanging chain is at the point <m>x=0</m> so that <m>y'(0) = 0</m>.        
    </p>
    
  </problem>





</section>